automate some Rows proofs

src/Experiments/SimplyTypedArithmetic.v
@@ -803,7 +803,41 @@ Module Columns.
   End Columns.
 End Columns.
 
+Module DivMod.
+  Definition is_div_mod {T} (evalf : T -> Z) dm y n :=
+    evalf (fst dm) = y mod n /\ snd dm = y / n. 
+
+  Lemma is_div_mod_step {T} evalf1 evalf2 dm1 dm2 y1 y2 n1 n2 x :
+    n1 > 0 ->
+    0 < n2 / n1 ->
+    n2 mod n1 = 0 ->
+    evalf2 (fst dm2) = evalf1 (fst dm1) + n1 * ((snd dm1 + x) mod (n2 / n1)) ->
+    snd dm2 = (snd dm1 + x) / (n2 / n1) ->
+    y2 = y1 + n1 * x ->
+    @is_div_mod T evalf1 dm1 y1 n1 ->
+    @is_div_mod T evalf2 dm2 y2 n2.
+  Proof.
+    intros; subst y2; cbv [is_div_mod] in *.
+    repeat match goal with
+           | H: _ /\ _ |- _ => destruct H
+           | H: ?LHS = _ |- _ => match LHS with context [dm2] => rewrite H end
+           | H: ?LHS = _ |- _ => match LHS with context [dm1] => rewrite H end
+           | _ => rewrite (Columns.flatten_mod_step (fun _ => 0)) by omega
+           | _ => rewrite (Columns.flatten_div_step (fun _ => 0)) by omega
+           | _ => rewrite Z.mul_div_eq_full by omega
+           end.
+    split; f_equal; omega.
+  Qed.
+
+  Lemma is_div_mod_result_equal {T} evalf dm y1 y2 n :
+    y1 = y2 ->
+    @is_div_mod T evalf dm y1 n ->
+    @is_div_mod T evalf dm y2 n.
+  Proof. congruence. Qed.
+End DivMod.
+
 Module Rows.
+  Import DivMod.
   Section Rows.
     Context (weight : nat->Z)
             {weight_0 : weight 0%nat = 1}
@@ -818,6 +852,7 @@ Module Rows.
     Hint Rewrite Positional.eval_nil Positional.eval0 @Positional.eval_snoc
          Columns.eval_nil Columns.eval_snoc using (auto; solve [distr_length]) : push_eval.
     Hint Resolve in_eq in_cons.
+    Hint Resolve Z.gt_lt.
 
     Definition eval n (inp : rows) :=
       sum (map (Positional.eval weight n) inp).
@@ -833,6 +868,16 @@ Module Rows.
     Lemma eval_app n x y : eval n (x ++ y) = eval n x + eval n y.
     Proof. cbv [eval]; autorewrite with push_map push_sum; reflexivity. Qed.
     Hint Rewrite eval_app : push_eval.
+
+    Ltac In_cases :=
+      repeat match goal with
+             | H: In _ (_ ++ _) |- _ => apply in_app_or in H; destruct H
+             | H: In _ (_ :: _) |- _ => apply in_inv in H; destruct H
+             | H: In _ nil |- _ => contradiction H
+             | H: forall x, In x (?y :: ?ls) -> ?P |- _ =>
+               unique pose proof (H y ltac:(apply in_eq));
+               unique assert (forall x, In x ls -> P) by auto
+             end.
 
     Section FromAssociational.
       (* extract row *)
@@ -899,13 +944,6 @@ Module Rows.
                    ) start_state (List.repeat 0 n).
 
       Definition from_columns (inp : cols) : rows := snd (from_columns' (max_column_size inp) (inp, [])).
-
-      Local Ltac In_cases :=
-        repeat match goal with
-               | H: In _ (_ ++ _) |- _ => apply in_app_or in H; destruct H
-               | H: In _ (_ :: _) |- _ => apply in_inv in H; destruct H
-               | H: In _ nil |- _ => contradiction H
-               end.
 
       Lemma eval_from_columns'_with_length m st n:
         (length (fst st) = n) ->
@@ -1015,62 +1053,66 @@ Module Rows.
                           (fst state ++ [fst sum_carry], snd sum_carry)) start_state (rev (combine row1 row2)).
         Definition sum_rows := sum_rows' (nil,0).
 
-        Lemma sum_rows'_div_mod_length row1 :
-          forall n m start_state row2 row1' row2',
-            length (fst start_state) = m -> length row1 = n -> length row2 = n ->
-            length row1' = m -> length row2' = m ->
-            let nm : nat := (n + m)%nat in
-            let eval := Positional.eval weight in
-            eval m (fst start_state) = (eval m row1' + eval m row2') mod (weight m) ->
-            snd start_state = (eval m row1' + eval m row2') / weight m ->
-            length (fst (sum_rows' start_state row1 row2)) = (n + m)%nat
-            /\ eval nm (fst (sum_rows' start_state row1 row2))
-               = (eval nm (row1' ++ row1) + eval nm (row2' ++ row2)) mod (weight nm)
-            /\ snd (sum_rows' start_state row1 row2) 
-               = (eval nm (row1' ++ row1) + eval nm (row2' ++ row2)) / (weight nm).
-        Proof.
-          cbv [sum_rows' Let_In].
-          induction row1 as [|x1 row1]; intros; rewrite fold_left_rev_right in *;
-            destruct row2 as [|x2 row2]; distr_length; [ subst n | ];
-              repeat match goal with
-                     | _ => progress autorewrite with natsimplify list
-                     | _ => progress cbn [fold_left combine]
-                     | _ => omega
-                     end.
+        Ltac push :=
+          repeat match goal with
+                 | _ => progress cbv [Let_In]
+                 | _ => rewrite Nat.add_1_r
+                 | _ => erewrite Positional.eval_snoc by eauto
+                 | H : length _ = _ |- _ => rewrite H
+                 | H: 0%nat = _ |- _ => rewrite <-H
+                 | p := _ |- _ => subst p
+                 | _ => progress autorewrite with cancel_pair natsimplify push_sum_rows list
+                 | _ => progress distr_length
+                 | _ => ring
+                 | _ => solve [ repeat (f_equal; try ring) ]
+                 | _ => tauto
+                 | _ => solve [eauto]
+                 end.
 
-          specialize (IHrow1 (pred n) (S m)).
-          replace (pred n + S m)%nat with (n + m)%nat in IHrow1 by omega.
+        Lemma sum_rows'_cons state x1 row1 x2 row2 :
+          sum_rows' state (x1 :: row1) (x2 :: row2) =
+          sum_rows' (fst state ++ [(snd state + x1 + x2) mod (fw (length (fst state)))], (snd state + x1 + x2) / fw (length (fst state))) row1 row2.
+        Proof.
+          cbv [sum_rows' Let_In]; autorewrite with push_combine.
+          rewrite !fold_left_rev_right. cbn [fold_left].
+          autorewrite with cancel_pair to_div_mod. congruence.
+        Qed.
+
+        Lemma sum_rows'_nil state :
+          sum_rows' state nil nil = state.
+        Proof. reflexivity. Qed.
+
+        Hint Rewrite sum_rows'_cons sum_rows'_nil : push_sum_rows.
+
+        Lemma sum_rows'_div_mod_length row1 :
+          forall nm start_state row2 row1' row2',
+            let m := length (fst start_state) in
+            let n := length row1 in
+            length row2 = n ->
+            length row1' = m ->
+            length row2' = m ->
+            (nm = n + m)%nat ->
+            let eval := Positional.eval weight in
+            is_div_mod (eval m) start_state (eval m row1' + eval m row2') (weight m) ->
+            length (fst (sum_rows' start_state row1 row2)) = nm
+            /\ is_div_mod (eval nm) (sum_rows' start_state row1 row2)
+                          (eval nm (row1' ++ row1) + eval nm (row2' ++ row2))
+                          (weight nm).
+        Proof.
+          induction row1 as [|x1 row1]; destruct row2 as [|x2 row2]; intros; subst nm; push.
           rewrite (app_cons_app_app _ row1'), (app_cons_app_app _ row2').
-          rewrite <-fold_left_rev_right.
-          apply IHrow1; clear IHrow1; autorewrite with cancel_pair distr_length; try omega;
-            repeat match goal with
-                   | H : ?LHS = _ |- _ =>
-                     match LHS with context [start_state] => rewrite H end
-                   | H : length _ = _ |- _ => rewrite H
-                   | _ => rewrite <-Z.div_add by auto
-                   | _ => rewrite Z.div_div by auto using Z.gt_lt
-                   | _ => rewrite Z.mul_div_eq by auto
-                   | _ => rewrite weight_multiples
-                   | _ => erewrite Positional.eval_snoc by eauto
-                   | _ => progress autorewrite with cancel_pair distr_length to_div_mod in *
-                   | |- context [ ?x mod ?m + ?m * (((?x + ?a * ?m + ?b * ?m)/ ?m) mod ?c) ] =>
-                     replace (x mod m) with ((x + a * m + b * m) mod m) by
-                         (autorewrite with zsimplify; ring);
-                       rewrite <-Z.rem_mul_r by auto using Z.gt_lt
-                   | _ => f_equal; ring
-                   end.
+          apply IHrow1; clear IHrow1; autorewrite with cancel_pair distr_length in *; try omega.
+          eapply is_div_mod_step with (x := x1 + x2); try eassumption; push.
         Qed.
         
         Lemma sum_rows_div_mod n row1 row2 :
           length row1 = n -> length row2 = n ->
           let eval := Positional.eval weight in
-          eval n (fst (sum_rows row1 row2)) = (eval n row1 + eval n row2) mod (weight n)
-          /\ snd (sum_rows row1 row2) = (eval n row1 + eval n row2) / (weight n).
+          is_div_mod (eval n) (sum_rows row1 row2) (eval n row1 + eval n row2) (weight n).
         Proof.
-          cbv [sum_rows]; intros. rewrite <-(Nat.add_0_r n).
-          edestruct sum_rows'_div_mod_length as [Hlen [Hmod  Hdiv] ];
-            try erewrite Hmod, Hdiv; auto using nil_length0;
-              autorewrite with cancel_pair push_eval zsimplify_fast; distr_length.
+          cbv [sum_rows]; intros.
+          apply sum_rows'_div_mod_length with (row1':=nil) (row2':=nil);
+            cbv [is_div_mod]; autorewrite with cancel_pair push_eval zsimplify; distr_length.
         Qed.
 
         Lemma sum_rows_mod n row1 row2 :
@@ -1153,21 +1195,23 @@ Module Rows.
           rewrite Z.div_0_l by auto; omega.
         Qed.
 
-        Lemma length_sum_rows row1 row2 n :
+        Lemma length_sum_rows row1 row2 n:
           length row1 = n -> length row2 = n ->
           length (fst (sum_rows row1 row2)) = n.
         Proof.
-          cbv [sum_rows]; intros. rewrite <-(Nat.add_0_r n).
-          eapply sum_rows'_div_mod_length; auto using nil_length0.
+          cbv [sum_rows]; intros.
+          eapply sum_rows'_div_mod_length; cbv [is_div_mod];
+            autorewrite with cancel_pair; distr_length; auto using nil_length0.
         Qed. Hint Rewrite length_sum_rows : distr_length.
       End SumRows.
+      Hint Resolve length_sum_rows.
       Hint Rewrite sum_rows_mod using (auto; solve [distr_length; auto]) : push_eval.
 
 
       Definition flatten' (start_state : list Z * Z) (inp : rows) : list Z * Z :=
         fold_right (fun next_row (state : list Z * Z)=>
                       let out_carry := sum_rows next_row (fst state) in
-                      (fst out_carry, snd state + snd out_carry)) start_state inp.
+                      (fst out_carry, snd state + snd out_carry)) start_state (rev inp).
 
       (* For correctness if there is only one row, we add a row of
          zeroes with the same length so that the add loop still happens. *)
@@ -1175,51 +1219,54 @@ Module Rows.
         let first_row := hd nil inp in
         flatten' (first_row, 0) (hd (Positional.zeros (length first_row)) (tl inp) :: tl (tl inp)).
 
+      (* TODO : move to ListUtil *)
+      Lemma rev_cons {A} x ls : @rev A (x :: ls) = rev ls ++ [x]. Proof. reflexivity. Qed. 
+      Hint Rewrite @rev_cons : list.
+      
       (* TODO: move to ListUtil *)
-      (* connect state to remaining input *)
-      Lemma fold_right_invariant_strong {A B} (P: list B -> A -> Type) (f: B -> A -> A):
-        forall bs a0
-               (Pnil : P nil a0)
-               (IHfold:
-                  forall bs' b a',
-                    In b bs ->
-                    a' = fold_right f a0 bs' ->
-                    P bs' a' ->
-                    P (b :: bs') (f b a')),
-          P bs (fold_right f a0 bs).
-      Proof. induction bs; intros; autorewrite with push_fold_right; auto using in_eq,in_cons. Qed.
+      Lemma fold_right_snoc {A B} f a x ls:
+        @fold_right A B f a (ls ++ [x]) = fold_right f (f x a) ls.
+      Proof.
+        rewrite <-(rev_involutive ls), <-rev_cons.
+        rewrite !fold_left_rev_right; reflexivity.
+      Qed.
+      Hint Rewrite @fold_right_snoc : push_fold_right.
+      
+      Lemma flatten'_cons state r inp :
+        flatten' state (r :: inp) = flatten' (fst (sum_rows r (fst state)), snd state + snd (sum_rows r (fst state))) inp.
+      Proof. cbv [flatten']; autorewrite with list push_fold_right. reflexivity. Qed.
+      Lemma flatten'_nil state : flatten' state [] = state. Proof. reflexivity. Qed.
+      Hint Rewrite flatten'_cons flatten'_nil : push_flatten.
 
-      Lemma flatten'_div_mod_length n start_state inp:
+      Ltac push :=
+        repeat match goal with
+               | _ => progress intros
+               | H: length ?x = ?n |- context [snd (sum_rows ?x _)] => rewrite sum_rows_div with (n:=n) by (distr_length; eauto)
+               | H: length ?x = ?n |- context [snd (sum_rows _ ?x)] => rewrite sum_rows_div with (n:=n) by (distr_length; eauto)
+               | H: length _ = _ |- _ => rewrite H
+               | _ => progress autorewrite with cancel_pair push_flatten push_eval distr_length zsimplify_fast
+               | _ => progress In_cases
+               | |- _ /\ _ => split
+               | |- context [?x mod ?y] => unique pose proof (Z.mul_div_eq_full x y ltac:(auto)); lia
+               | _ => solve [repeat (f_equal; try ring)]
+               | _ => congruence
+               | _ => solve [eauto]
+               end.
+
+      Lemma flatten'_div_mod_length n inp : forall start_state,
         length (fst start_state) = n ->
         (forall row, In row inp -> length row = n) ->
         length (fst (flatten' start_state inp)) = n
         /\ (inp <> nil ->
-            Positional.eval weight n (fst (flatten' start_state inp)) = (Positional.eval weight n (fst start_state) + eval n inp) mod (weight n)
-            /\ snd (flatten' start_state inp) = snd start_state + (Positional.eval weight n (fst start_state) + eval n inp) / weight n).
+            is_div_mod (Positional.eval weight n) (flatten' start_state inp)
+                       (Positional.eval weight n (fst start_state) + eval n inp + weight n * snd start_state)
+                       (weight n)).
       Proof.
-        intro.
-        cbv [flatten'].
-        apply fold_right_invariant_strong with (bs:=inp); intros; [ tauto | destruct (dec (bs' = nil)) ];
-          repeat match goal with
-                 | _ => subst a'
-                 | _ => subst bs'
-                 | _ => rewrite sum_rows_div with (n:=n) by auto
-                 | _ => rewrite @fold_right_nil in *
-                 | _ => progress autorewrite with cancel_pair push_eval in *
-                 | H : _ -> _ /\ _ |- _ =>
-                   let X := fresh in let Y := fresh in
-                                     destruct H as [X Y]; [ solve [auto using in_cons] | rewrite ?X, ?Y ]
-                 | _ => split
-                 | _ => progress autorewrite with pull_Zmod zsimplify_fast
-                 | _ => solve [ auto using length_sum_rows ]
-                 | _ => solve [ ring_simplify; repeat (f_equal; try ring) ]
-                 end.
-        apply Z.mul_cancel_l with (p:=weight n); [ apply weight_nonzero |].
-        autorewrite with push_Zmul.
-        rewrite !Z.mul_div_eq_full by apply weight_nonzero.
-        autorewrite with pull_Zmod.
-        ring_simplify_subterms. ring_simplify.
-        repeat (f_equal; try ring).
+        induction inp; push; [apply IHinp; push|].
+        destruct (dec (inp = nil)); [subst inp; cbv [is_div_mod]
+                                    | eapply is_div_mod_result_equal; try apply IHinp]; push.
+        { autorewrite with zsimplify; push. }
+        { autorewrite with zsimplify; push. }
       Qed.
 
       Hint Rewrite (@Positional.length_zeros weight) : distr_length.
@@ -1227,22 +1274,11 @@ Module Rows.
 
       Lemma flatten_div_mod inp n :
         (forall row, In row inp -> length row = n) ->
-        Positional.eval weight n (fst (flatten inp)) = (eval n inp) mod (weight n)
-        /\ snd (flatten inp) = (eval n inp) / weight n.
+        is_div_mod (Positional.eval weight n) (flatten inp) (eval n inp) (weight n).
       Proof.
         intros; cbv [flatten].
-        destruct inp; [|destruct inp]; cbn [hd tl].
-        { cbn. autorewrite with push_eval. tauto. }
-        { cbn.
-          match goal with H : forall r, In r [?x] -> _ |- _ =>
-                          specialize (H x ltac:(auto)); rewrite H
-          end.
-          rewrite sum_rows_div with (n:=n) by distr_length.
-          autorewrite with push_eval.
-          split; f_equal; ring. }
-        { autorewrite with push_eval.
-          apply flatten'_div_mod_length; auto.
-          congruence. }
+        destruct inp; [|destruct inp]; cbn [hd tl]; try solve [cbv [is_div_mod]; push].
+        eapply is_div_mod_result_equal; try apply flatten'_div_mod_length; push.
       Qed.
 
       Lemma flatten_mod inp n :
@@ -1266,25 +1302,24 @@ Module Rows.
         inp <> nil ->
         length (fst (flatten inp)) = n.
       Proof.
-        intros.
-        destruct inp; [congruence |]; destruct inp;
-          repeat match goal with
-                 | _ => progress intros
-                 | _ => progress cbn [hd tl] in *
-                 | _ => progress autorewrite with cancel_pair
-                 | _ => apply flatten'_div_mod_length
-                 | H: _ |- _ => apply in_inv in H; destruct H
-                 | _ => solve [auto]
-                 end;
-          subst row; distr_length; auto.
+        intros. apply flatten'_div_mod_length; push;
+          destruct inp as [|? [|? ?] ]; try congruence; cbn [hd tl] in *; push.
+        subst row; distr_length; auto.
       Qed. Hint Rewrite length_flatten : distr_length.
 
-      Lemma flatten'_cons state x inp :
-        flatten' state (x :: inp)
-        = (fst (sum_rows x (fst (flatten' state inp))), snd (flatten' state inp) + snd (sum_rows x (fst (flatten' state inp)))).
-      Proof. reflexivity. Qed.
+      (* TODO: move to ZUtil *)
+      Lemma add_mod_l_multiple a b n m:
+        0 < n / m -> m <> 0 -> n mod m = 0 ->
+        (a mod n + b) mod m = (a + b) mod m.
+      Proof.
+        intros.
+        rewrite (proj2 (Z.div_exact n m ltac:(auto))) by auto.
+        rewrite Z.rem_mul_r by auto.
+        push_Zmod. autorewrite with zsimplify.
+        pull_Zmod. reflexivity.
+      Qed.
       
-      Lemma flatten'_partitions n start_state inp:
+      Lemma flatten'_partitions n inp : forall start_state,
         length (fst start_state) = n ->
         (forall row, In row inp -> length row = n) ->
         inp <> nil ->
@@ -1292,18 +1327,11 @@ Module Rows.
                   nth_default 0 (fst (flatten' start_state inp)) i
                   = ((Positional.eval weight n (fst start_state) + eval n inp) mod weight (S i)) / (weight i).
       Proof.
-        intro.
-        induction inp; intros; [congruence|].
-        rewrite flatten'_cons.
-        autorewrite with push_fold_right cancel_pair.
-        rewrite sum_rows_partitions with (n:=n) by (rewrite ?length_flatten' with (n:=n); auto).
+        induction inp; push.
         destruct (dec (inp = nil)).
-        { subst inp. cbn. repeat (f_equal; try ring). }
-        { edestruct flatten'_div_mod_length with (inp:=inp) as [Hlen [Hmod Hdiv] ]; eauto.
-          rewrite Hmod. autorewrite with push_eval.
-          rewrite Z.add_mod_full. erewrite @Columns.weight_div_mod with (j:=n) (i:=S i) by eauto.
-          rewrite Z.rem_mul_r by auto using Z.gt_lt, weight_divides_full.
-          autorewrite with zsimplify. pull_Zmod.
+        { subst inp; push. rewrite sum_rows_partitions with (n:=n) by eauto. push. }
+        { erewrite IHinp; push.
+          rewrite add_mod_l_multiple by auto using weight_divides_full, Columns.weight_multiples_full.
           repeat (f_equal; try ring). }
       Qed.
 
@@ -1313,18 +1341,10 @@ Module Rows.
                   nth_default 0 (fst (flatten inp)) i = (eval n inp mod weight (S i)) / (weight i).
       Proof.
         intros; cbv [flatten].
-        destruct inp; [|destruct inp]; cbn [hd tl].
-        { cbn. autorewrite with push_eval push_nth_default zsimplify. reflexivity. }
-        { cbn.
-          match goal with H : forall r, In r [?x] -> _ |- _ =>
-                          specialize (H x ltac:(auto)); rewrite H
-          end.
-          rewrite sum_rows_partitions with (n:=n) by distr_length.
-          autorewrite with push_eval.
-          repeat (f_equal; try ring). }
-        { autorewrite with push_eval.
-          apply flatten'_partitions; auto.
-          congruence. }
+        intros; destruct inp as [| ? [| ? ?] ]; try congruence; cbn [hd tl] in *;  try solve [push].
+        { cbn. autorewrite with push_nth_default. reflexivity. }
+        { push. rewrite sum_rows_partitions with (n:=n) by distr_length; push. }
+        { rewrite flatten'_partitions with (n:=n); push. }
       Qed.
     End Flatten.
 
